src/Symbolic/Expr/CmpSmartInfo.v
@@ -1,58 +1,327 @@
 Require Import CoqStock.List.
 Require Export CoqStock.Cmp.
+Require Import CoqStock.CmpNat.
+Require Import CoqStock.DubStep.
 
-Require Import Symbolic.Expr.CmpInfo.
+Require Import Symbolic.Expr.Info.
 Require Import Symbolic.Expr.SmartInfo.
 
-Fixpoint compare_smart_info (x y: SmartInfo) {struct x} :=
+Fixpoint compare_info (x y: Info) {struct x}: comparison :=
   match x with
-  | mkSmart x' _ =>
+  | mkInfo xname xparams _ xhash =>
     match y with
-    | mkSmart y' _ =>
-      CmpInfo.compare_info x' y'
+    | mkInfo yname yparams _ yhash =>
+      match compare xhash yhash with
+      | Lt => Lt
+      | Gt => Gt
+      | Eq =>
+        match compare xname yname with
+        | Lt => Lt
+        | Gt => Gt
+        | Eq => ((fix compare_params (xs ys: list Info) {struct xs} :=
+        (match xs with
+         | [] =>
+           match ys with
+           | [] => Eq
+           | _ => Lt
+           end
+         | (x'::xs') =>
+           match ys with
+           | [] => Gt
+           | (y'::ys') =>
+             match compare_info x' y' with
+             | Lt => Lt
+             | Gt => Gt
+             | Eq => compare_params xs' ys'
+             end
+           end
+         end)) xparams yparams)
+        end
+      end
+    end
+  end
+.
+
+Definition compare_smart_info (xsmart ysmart: SmartInfo): comparison :=
+  match xsmart with
+  | mkSmart xinfo x_is_smart =>
+    match ysmart with
+    | mkSmart yinfo y_is_smart =>
+      compare_info xinfo yinfo
     end
   end.
 
-Theorem proof_info_compare_eq_implies_equal: forall (x y: Info)
-  (c: compare_info x y = Eq)
+(* Fixpoint compare_smart_info (xsmart ysmart: SmartInfo) {struct xsmart}: comparison.
+specialize (get_smart_params xsmart) as xsmartparams.
+specialize (get_smart_params ysmart) as ysmartparams.
+destruct xsmart as [xinfo x_is_smart].
+destruct ysmart as [yinfo y_is_smart].
+destruct xinfo as [xname xparams xhasvar xhash].
+destruct yinfo as [yname yparams yhasvar yhash].
+destruct x_is_smart as [x_smart_hasvar x_smart_hash].
+destruct y_is_smart as [y_smart_hasvar y_smart_hash].
+destruct x_smart_hasvar as [x_smart_hasvar' x_smart_hasvars].
+
+
+
+  match xsmart with
+  | mkSmart xinfo x_is_smart =>
+    match ysmart with
+    | mkSmart yinfo y_is_smart =>
+      match xinfo as xinfo' return (IsSmart xinfo' -> comparison) with
+      | mkInfo xname xparams xhasvar xhash =>
+        (fun (xsmart: IsSmart (mkInfo xname xparams xhasvar xhash)) =>
+          match yinfo as yinfo' return (IsSmart yinfo' -> comparison) with
+          | mkInfo yname yparams yhasvar yhash =>
+            (fun (ysmart: IsSmart (mkInfo yname yparams yhasvar yhash)) =>
+              Eq
+            )
+          end y_is_smart
+        )
+      end x_is_smart
+    end
+  end.
+
+Fixpoint compare_smart_info (xsmart ysmart: SmartInfo) {struct xsmart}: comparison :=
+  match xsmart with
+  | mkSmart xinfo x_is_smart =>
+    match ysmart with
+    | mkSmart yinfo y_is_smart =>
+      match xinfo as xinfo' return (IsSmart xinfo' -> comparison) with
+      | mkInfo xname xparams xhasvar xhash =>
+        (fun (xsmart: IsSmart (mkInfo xname xparams xhasvar xhash)) =>
+          match yinfo as yinfo' return (IsSmart yinfo' -> comparison) with
+          | mkInfo yname yparams yhasvar yhash =>
+            (fun (ysmart: IsSmart (mkInfo yname yparams yhasvar yhash)) =>
+              Eq
+            )
+          end y_is_smart
+        )
+      end x_is_smart
+    end
+  end.
+
+
+Definition get_sparams (s : SmartInfo): list SmartInfo :=
+  match s with
+  | mkSmart info smart =>
+     match info as i return (IsSmart i -> list SmartInfo) with
+     | mkInfo name params hasvar hash =>
+         (fun
+            (smart1 : IsSmart (mkInfo name params hasvar hash)) =>
+          match smart1 with
+          | isSmart _ x x0 =>
+              (fun
+                 (smartHasVar : IsSmartHasVar
+                                  (mkInfo name params hasvar hash))
+                 (smartHash : IsSmartHash
+                                (mkInfo name params hasvar hash)) =>
+               match smartHash with
+               | isSmartHash _ x1 x2 =>
+                   (fun
+                      (_ : get_hash (mkInfo name params hasvar hash) =
+                           hash_from_info
+                             (mkInfo name params hasvar hash))
+                      (smartHashes : Forall IsSmartHash
+                                       (get_params
+                                          (mkInfo name params hasvar hash)))
+                    =>
+                    match smartHasVar with
+                    | isSmartHasVar _ x3 x4 =>
+                        (fun
+                           (_ : get_hasvar
+                                  (mkInfo name params hasvar hash) = true \/
+                                get_hasvar
+                                  (mkInfo name params hasvar hash) =
+                                has_var_from_params
+                                  (get_params
+                                     (mkInfo name params hasvar hash)))
+                           (smartHasVars : Forall IsSmartHasVar
+                                             (get_params
+                                                (mkInfo name params hasvar
+                                                 hash))) =>
+                         get_smart_params' params smartHasVars smartHashes)
+                          x3 x4
+                    end) x1 x2
+               end) x x0
+          end)
+     end smart
+end.
+
+
+Definition get_sparams (s : SmartInfo): list SmartInfo :=
+  match s with
+  | mkSmart info smart =>
+  (fun (info0 : Info) (smart0 : IsSmart info0) =>
+     match info0 as i return (IsSmart i -> list SmartInfo) with
+     | mkInfo name params hasvar hash =>
+         (fun (name0 : nat) (params0 : list Info)
+            (hasvar0 : bool) (hash0 : nat)
+            (smart1 : IsSmart (mkInfo name0 params0 hasvar0 hash0)) =>
+          match smart1 with
+          | isSmart _ x x0 =>
+              (fun
+                 (smartHasVar : IsSmartHasVar
+                                  (mkInfo name0 params0 hasvar0 hash0))
+                 (smartHash : IsSmartHash
+                                (mkInfo name0 params0 hasvar0 hash0)) =>
+               match smartHash with
+               | isSmartHash _ x1 x2 =>
+                   (fun
+                      (_ : get_hash (mkInfo name0 params0 hasvar0 hash0) =
+                           hash_from_info
+                             (mkInfo name0 params0 hasvar0 hash0))
+                      (smartHashes : Forall IsSmartHash
+                                       (get_params
+                                          (mkInfo name0 params0 hasvar0 hash0)))
+                    =>
+                    match smartHasVar with
+                    | isSmartHasVar _ x3 x4 =>
+                        (fun
+                           (_ : get_hasvar
+                                  (mkInfo name0 params0 hasvar0 hash0) = true \/
+                                get_hasvar
+                                  (mkInfo name0 params0 hasvar0 hash0) =
+                                has_var_from_params
+                                  (get_params
+                                     (mkInfo name0 params0 hasvar0 hash0)))
+                           (smartHasVars : Forall IsSmartHasVar
+                                             (get_params
+                                                (mkInfo name0 params0 hasvar0
+                                                 hash0))) =>
+                         get_smart_params' params0 smartHasVars smartHashes)
+                          x3 x4
+                    end) x1 x2
+               end) x x0
+          end) name params hasvar hash
+     end smart0) info smart
+end.
+
+
+Fixpoint compare_smart_info (xsmart ysmart: SmartInfo) {struct xsmart} :=
+  match xsmart with
+  | mkSmart xinfo x_is_smart =>
+    match ysmart with
+    | mkSmart yinfo y_is_smart =>
+      match xinfo with
+      | mkInfo xname xparams _ xhash =>
+        match yinfo with
+        | mkInfo yname yparams _ yhash =>
+          match Nat.compare xhash yhash with
+          | Lt => Lt
+          | Gt => Gt
+          | Eq =>
+            match Nat.compare xname yname with
+            | Lt => Lt
+            | Gt => Gt
+            | Eq => ((fix compare_params (xs ys: list SmartInfo) {struct xs} :=
+              (match xs with
+              | [] =>
+                match ys with
+                | [] => Eq
+                | _ => Lt
+                end
+              | (x'::xs') =>
+                match ys with
+                | [] => Gt
+                | (y'::ys') =>
+                  match compare_smart_info x' y' with
+                  | Lt => Lt
+                  | Gt => Gt
+                  | Eq => compare_params xs' ys'
+                  end
+                end
+              end)) (get_smart_params xsmart) (get_smart_params ysmart))
+            end
+          end
+        end
+      end
+    end
+  end.
+
+Print compare_smart_info.
+ *)
+
+
+Theorem proof_compare_smart_info_eq_implies_equal: forall (x y: SmartInfo)
+  (c: compare_smart_info x y = Eq)
   , x = y.
 Proof.
+destruct x as [xinfo x_is_smart].
+destruct y as [yinfo y_is_smart].
+destruct xinfo as [xname xparams xhasvar xhash].
+destruct yinfo as [yname yparams yhasvar yhash].
+destruct x_is_smart as [x_smart_hasvar x_smart_hash].
+destruct y_is_smart as [y_smart_hasvar y_smart_hash].
+destruct x_smart_hasvar as [x_smart_hasvar' x_smart_hasvars].
+destruct y_smart_hasvar as [y_smart_hasvar' y_smart_hasvars].
+destruct x_smart_hash as [x_smart_hash' x_smart_hashes].
+destruct y_smart_hash as [y_smart_hash' y_smart_hashes].
+unfold compare_smart_info.
+dubstep compare_info.
+intros.
+induction_on_compare.
+subst.
+induction_on_compare.
+subst.
+induction xparams.
+- cbn in x_smart_hashes.
+  induction yparams.
+    cbn in y_smart_hashes.
+    destruct xhasvar, yhasvar.
+    * cbn in x_smart_hasvars.
+      cbn in y_smart_hasvars.
+      rewrite (Forall_nil_iff IsSmartHash) in x_smart_hashes.
+      destruct x_smart_hashes.
+      --- admit.
+      ---
+remember (compare xhash yhash).
+induction c0.
+
+rewrite_nat_compare_to_compare.
+
+
+rewrite_nat_compare_to_compare.
+induction_on_compare.
+
+intros.
+
 (*TODO*)
 Admitted.
 
-Theorem proof_info_compare_eq_reflex: forall (p: Info)
-  , compare_info p p = Eq.
+Theorem proof_compare_smart_info_eq_reflex: forall (p: SmartInfo)
+  , compare_smart_info p p = Eq.
 (*TODO*)
 Admitted.
 
-Theorem proof_info_compare_eq_trans: forall (x y z: Info)
-  (xy: compare_info x y = Eq)
-  (yz: compare_info y z = Eq)
-  , compare_info x z = Eq.
+Theorem proof_compare_smart_info_eq_trans: forall (x y z: SmartInfo)
+  (xy: compare_smart_info x y = Eq)
+  (yz: compare_smart_info y z = Eq)
+  , compare_smart_info x z = Eq.
 (*TODO*)
 Admitted.
 
-Theorem proof_info_compare_lt_trans: forall (x y z: Info)
-  (xy: compare_info x y = Lt)
-  (yz: compare_info y z = Lt)
-  , compare_info x z = Lt.
+Theorem proof_compare_smart_info_lt_trans: forall (x y z: SmartInfo)
+  (xy: compare_smart_info x y = Lt)
+  (yz: compare_smart_info y z = Lt)
+  , compare_smart_info x z = Lt.
 (*TODO*)
 Admitted.
 
-Theorem proof_info_compare_gt_trans: forall (x y z: Info)
-  (xy: compare_info x y = Gt)
-  (yz: compare_info y z = Gt)
-  , compare_info x z = Gt.
+Theorem proof_compare_smart_info_gt_trans: forall (x y z: SmartInfo)
+  (xy: compare_smart_info x y = Gt)
+  (yz: compare_smart_info y z = Gt)
+  , compare_smart_info x z = Gt.
 (*TODO*)
 Admitted.
 
 #[export]
-Instance CmpInfo: Cmp (Info) :=
+Instance CmpSmartInfo: Cmp (SmartInfo) :=
   {
-    compare := compare_info
-  ; proof_compare_eq_implies_equal := proof_info_compare_eq_implies_equal
-  ; proof_compare_eq_reflex := proof_info_compare_eq_reflex
-  ; proof_compare_eq_trans := proof_info_compare_eq_trans
-  ; proof_compare_lt_trans := proof_info_compare_lt_trans
-  ; proof_compare_gt_trans := proof_info_compare_gt_trans
+    compare := compare_smart_info
+  ; proof_compare_eq_implies_equal := proof_compare_smart_info_eq_implies_equal
+  ; proof_compare_eq_reflex := proof_compare_smart_info_eq_reflex
+  ; proof_compare_eq_trans := proof_compare_smart_info_eq_trans
+  ; proof_compare_lt_trans := proof_compare_smart_info_lt_trans
+  ; proof_compare_gt_trans := proof_compare_smart_info_gt_trans
   }.
