src/CoqStock/ForAll.v
@@ -1,0 +1,6 @@
+(* Musketeers One for all *)
+
+Require Import CoqStock.List.
+
+Definition ForAll {A: Set} (P: A -> Prop) (xs: list A): Prop :=
+  fold_left (fun p x => p /\ (P x)) xs True.
